theories/base.v
@@ -136,3 +136,72 @@ Proof.
   iExists (x::xs) => /=. iSplit; [by rewrite /= Heq|]. iFrame.
   iExists _. by iFrame.
 Qed.
+
+(** fixpoints based on iris/bi/lib/fixpoint.v *)
+Class MonoPred {A : Type} (F : (A → Prop) → (A → Prop)) := {
+  mono_pred (Φ Ψ : _ → Prop) :
+    (∀ x, Φ x → Ψ x) → ∀ x, F Φ x → F Ψ x;
+}.
+Global Arguments mono_pred {_ _ _} _ _.
+
+Definition least_fixpoint {A : Type}
+    (F : (A → Prop) → (A → Prop)) (x : A) : Prop :=
+  tc_opaque (∀ Φ : A -> Prop, (∀ x, F Φ x → Φ x) → Φ x).
+Global Arguments least_fixpoint : simpl never.
+Definition greatest_fixpoint {A : Type}
+    (F : (A → Prop) → (A → Prop)) (x : A) : Prop :=
+  tc_opaque (∃ Φ : A -> Prop, (∀ x, Φ x → F Φ x) ∧ Φ x).
+Global Arguments greatest_fixpoint : simpl never.
+
+Section least.
+  Context {A : Type} (F : (A → Prop) → (A → Prop)) `{!MonoPred F}.
+
+  Lemma least_fixpoint_unfold_2 x : F (least_fixpoint F) x → least_fixpoint F x.
+  Proof using Type*.
+    rewrite /least_fixpoint /=. move => HF Φ Hincl.
+    apply Hincl. apply: mono_pred; [|done].
+    move => /= y Hy. apply Hy. done.
+  Qed.
+
+  Lemma least_fixpoint_unfold_1 x : least_fixpoint F x → F (least_fixpoint F) x.
+  Proof using Type*.
+    move => HF. apply HF. move => y Hy /=. apply: mono_pred; [|done].
+    move => z Hz. by apply: least_fixpoint_unfold_2.
+  Qed.
+
+  Lemma least_fixpoint_unfold x : least_fixpoint F x ↔ F (least_fixpoint F) x.
+  Proof using Type*. split; eauto using least_fixpoint_unfold_1, least_fixpoint_unfold_2. Qed.
+
+  Lemma least_fixpoint_ind (Φ : A → Prop) :
+    (∀ y, F Φ y → Φ y) → ∀ x, least_fixpoint F x → Φ x.
+  Proof. move => HΦ x HF. by apply: HF. Qed.
+End least.
+
+Section greatest.
+  Context {A : Type} (F : (A → Prop) → (A → Prop)) `{!MonoPred F}.
+
+  Lemma greatest_fixpoint_unfold_1 x :
+    greatest_fixpoint F x → F (greatest_fixpoint F) x.
+  Proof using Type*.
+    move => [Φ [Hincl HΦ]].
+    apply: (mono_pred Φ); [| by apply: Hincl].
+    move => y Hy. eexists Φ. naive_solver.
+  Qed.
+
+  Lemma greatest_fixpoint_unfold_2 x :
+    F (greatest_fixpoint F) x → greatest_fixpoint F x.
+  Proof using Type*.
+    move => HF. eexists (F (greatest_fixpoint F)). split; [|done].
+    move => y Hy. apply: mono_pred; [|done]. move => z. apply: greatest_fixpoint_unfold_1.
+  Qed.
+
+  Corollary greatest_fixpoint_unfold x :
+    greatest_fixpoint F x ↔ F (greatest_fixpoint F) x.
+  Proof using Type*.
+    split; auto using greatest_fixpoint_unfold_1, greatest_fixpoint_unfold_2.
+  Qed.
+
+  Lemma greatest_fixpoint_coind (Φ : A → Prop) :
+    (∀ y, Φ y → F Φ y) → ∀ x, Φ x → greatest_fixpoint F x.
+  Proof. move => HΦ x Hx. eexists Φ. naive_solver. Qed.
+End greatest.
