examples/uart.v
@@ -1,0 +1,125 @@
+Require Import isla.isla.
+From isla.instructions.uart Require Import instrs.
+
+Section proof.
+Context `{!islaG Σ} `{!threadG}.
+
+Definition bus_to_reg32 (b : Z) : Z :=
+  b - 0x3f000000.
+Definition AUX_MU_LSR_REG : addr := [BV{64} bus_to_reg32 0x7e215054].
+Definition AUX_MU_IO_REG : addr := [BV{64} bus_to_reg32 0x7e215040].
+
+Definition spec_uart_wait_write_body (P R : spec) : spec :=
+  sexists (λ b : bv 32, scons (SReadMem AUX_MU_LSR_REG b)
+                              (sif (Z.testbit (bv_unsigned b) 5 = true) P R)).
+Global Instance spec_uart_wait_write_body_mono P :
+  MonoPred (spec_uart_wait_write_body P).
+Proof. constructor. unfold spec_uart_wait_write_body. by unshelve spec_solver. Qed.
+
+Definition spec_uart_wait_write (P : spec) : spec :=
+  srec (spec_uart_wait_write_body P).
+
+Definition spec_uart_write (c : bv 32) (P : spec) : spec :=
+  spec_uart_wait_write (scons (SWriteMem AUX_MU_IO_REG c) P).
+
+Definition uart1_putc_loop_spec : iProp Σ :=
+  ∃ P,
+  "R1" ↦ᵣ: λ _,
+  "R2" ↦ᵣ RVal_Bits AUX_MU_LSR_REG ∗
+  mmio_range AUX_MU_LSR_REG 0x4 ∗
+  reg_col sys_regs ∗
+  spec_trace (spec_uart_wait_write P) ∗
+  instr_pre 0x000000000008018c (
+    ∃ r1,
+    "R1" ↦ᵣ RVal_Bits r1 ∗
+    "R2" ↦ᵣ RVal_Bits AUX_MU_LSR_REG ∗
+    reg_col sys_regs ∗
+    spec_trace P ∗
+    True
+  )
+.
+Global Instance : LithiumUnfold (uart1_putc_loop_spec) := I.
+
+Lemma uart1_putc_loop :
+  instr 0x0000000000080180 (Some a80180) -∗
+  instr 0x0000000000080184 (Some a80184) -∗
+  instr 0x0000000000080188 (Some a80188) -∗
+  □ instr_pre 0x0000000000080180 uart1_putc_loop_spec -∗
+  instr_body 0x0000000000080180 uart1_putc_loop_spec.
+Proof.
+  iStartProof.
+  Time repeat liAStep; liShow.
+  liInst Hevar P.
+  Time repeat liAStep; liShow.
+
+  Unshelve. all: prepare_sidecond.
+  - bv_solve.
+  - rename select (_ ≠ _) into Hn.
+    rewrite sif_true; [done|]. apply not_false_is_true.
+    contradict Hn. bits_simplify. have -> : n1 = 0 by lia. done.
+  - rename select (_ = _) into Hn.
+    rewrite sif_false; [done|]. apply not_true_iff_false.
+    bitify_hyp Hn. move: (Hn 0 ltac:(done)) => {}Hn.
+    by bits_simplify_hyp Hn.
+Time Qed.
+
+Definition uart1_putc_spec : iProp Σ :=
+  ∃ P (c ret : bv 64),
+  "R0" ↦ᵣ RVal_Bits c ∗
+  "R1" ↦ᵣ: λ _,
+  "R2" ↦ᵣ: λ _,
+  "R30" ↦ᵣ RVal_Bits ret ∗
+  mmio_range AUX_MU_LSR_REG 0x4 ∗
+  mmio_range AUX_MU_IO_REG 0x4 ∗
+  reg_col sys_regs ∗
+  spec_trace (spec_uart_write (bv_zero_extend 32 (bv_extract 0 8 c)) P) ∗
+  instr_pre (bv_unsigned ret) (
+    ∃ r0 r1 r2 : bv 64,
+    "R0" ↦ᵣ RVal_Bits r0 ∗
+    "R1" ↦ᵣ RVal_Bits r1 ∗
+    "R2" ↦ᵣ RVal_Bits r2 ∗
+    reg_col sys_regs ∗
+    spec_trace P ∗
+    True
+  )
+.
+Global Instance : LithiumUnfold (uart1_putc_spec) := I.
+
+Lemma uart1_putc :
+  instr 0x0000000000080168 (Some a80168) -∗
+  instr 0x000000000008016c (Some a8016c) -∗
+  instr 0x0000000000080170 (Some a80170) -∗
+  instr 0x0000000000080174 (Some a80174) -∗
+  instr 0x0000000000080178 (Some a80178) -∗
+  instr 0x000000000008017c (Some a8017c) -∗
+  □ instr_pre 0x0000000000080180 uart1_putc_loop_spec -∗
+  instr 0x000000000008018c (Some a8018c) -∗
+  instr 0x0000000000080190 (Some a80190) -∗
+  instr 0x0000000000080194 (Some a80194) -∗
+  instr 0x0000000000080198 (Some a80198) -∗
+
+  instr_body 0x0000000000080168 (uart1_putc_spec).
+Proof.
+  iStartProof.
+  Time repeat liAStep; liShow.
+  have -> : LET3 = AUX_MU_LSR_REG by apply/bv_eq; done.
+  Time repeat liAStep; liShow.
+  - have -> : LET11 = AUX_MU_IO_REG by apply/bv_eq; done.
+    Time repeat liAStep; liShow.
+    rewrite sif_true; [|li_shelve_sidecond].
+    Time repeat liAStep; liShow.
+  - rewrite sif_false; [|li_shelve_sidecond].
+    liInst Hevar (scons (SWriteMem AUX_MU_IO_REG (bv_zero_extend 32 (bv_extract 0 8 c))) P).
+    Time repeat liAStep; liShow.
+    have -> : LET10 = AUX_MU_IO_REG by apply/bv_eq; done.
+    Time repeat liAStep; liShow.
+  Unshelve. all: prepare_sidecond.
+  all: try by bits_simplify.
+  + apply/bv_eq. done.
+  + rename select (_ = [BV{1} 1]) into Hn.
+    bitify_hyp Hn. move: (Hn 0 ltac:(done)) => {}Hn.
+    by bits_simplify_hyp Hn.
+  + rename select (_ ≠ [BV{1} 1]) into Hn. contradict Hn. bits_simplify.
+    by have -> : n1 = 0 by lia.
+Time Qed.
+End proof.
