instructions/uart/a80168.v
@@ -1,0 +1,8 @@
+From isla Require Import isla_lang.
+
+Definition a80168 : list trc := [
+  [
+    AssumeReg "__v85_implemented" [] (RegVal_Base (Val_Bool false)) Mk_annot;
+    WriteReg "R2" [] (RegVal_Base (Val_Bits [BV{64%N} 0x5054%Z])) Mk_annot
+  ]
+].
