instructions/uart/a80170.v
@@ -1,0 +1,11 @@
+From isla Require Import isla_lang.
+
+Definition a80170 : list trc := [
+  [
+    AssumeReg "__v85_implemented" [] (RegVal_Base (Val_Bool false)) Mk_annot;
+    Smt (DeclareConst 44%Z (Ty_BitVec 64%N)) Mk_annot;
+    ReadReg "R2" [] (RegVal_Base (Val_Symbolic 44%Z)) Mk_annot;
+    Smt (DefineConst 47%Z (Manyop (Bvmanyarith Bvor) [Manyop (Bvmanyarith Bvand) [Val (Val_Symbolic 44%Z) Mk_annot; Val (Val_Bits [BV{64%N} 0xffffffff0000ffff%Z]) Mk_annot] Mk_annot; Val (Val_Bits [BV{64%N} 0x3f210000%Z]) Mk_annot] Mk_annot)) Mk_annot;
+    WriteReg "R2" [] (RegVal_Base (Val_Symbolic 47%Z)) Mk_annot
+  ]
+].
