instructions/uart/a8019c.v
@@ -1,0 +1,7 @@
+From isla Require Import isla_lang.
+
+Definition a8019c : list trc := [
+  [
+    AssumeReg "__v85_implemented" [] (RegVal_Base (Val_Bool false)) Mk_annot
+  ]
+].
