instructions/uart/instrs.v
@@ -1,0 +1,32 @@
+Require Import isla.isla_lang.
+Require Export isla.instructions.uart.a80168.
+Require Export isla.instructions.uart.a8016c.
+Require Export isla.instructions.uart.a80170.
+Require Export isla.instructions.uart.a80174.
+Require Export isla.instructions.uart.a80178.
+Require Export isla.instructions.uart.a8017c.
+Require Export isla.instructions.uart.a80180.
+Require Export isla.instructions.uart.a80184.
+Require Export isla.instructions.uart.a80188.
+Require Export isla.instructions.uart.a8018c.
+Require Export isla.instructions.uart.a80190.
+Require Export isla.instructions.uart.a80194.
+Require Export isla.instructions.uart.a80198.
+Require Export isla.instructions.uart.a8019c.
+
+Definition instr_map := [
+  (0x80168%Z, a80168 (* mov x2, #0x5054 *));
+  (0x8016c%Z, a8016c (* and w0, w0, #0xff *));
+  (0x80170%Z, a80170 (* movk x2, #0x3f21, lsl #16 *));
+  (0x80174%Z, a80174 (* ldr w1, [x2] *));
+  (0x80178%Z, a80178 (* tbnz w1, #5, 8018c <uart1_putc+0x24> *));
+  (0x8017c%Z, a8017c (* nop *));
+  (0x80180%Z, a80180 (* nop *));
+  (0x80184%Z, a80184 (* ldr w1, [x2] *));
+  (0x80188%Z, a80188 (* tbz w1, #5, 80180 <uart1_putc+0x18> *));
+  (0x8018c%Z, a8018c (* mov x1, #0x5040 *));
+  (0x80190%Z, a80190 (* movk x1, #0x3f21, lsl #16 *));
+  (0x80194%Z, a80194 (* str w0, [x1] *));
+  (0x80198%Z, a80198 (* ret *));
+  (0x8019c%Z, a8019c (* nop *))
+].
