theories/spec.v
@@ -1,0 +1,63 @@
+Require Import refinedc.lithium.infrastructure.
+Require Import refinedc.lithium.simpl_classes.
+Require Import isla.opsem.
+
+Definition spec := list seq_label → Prop.
+
+Global Instance spec_subseteq : SubsetEq spec := λ P1 P2, ∀ κs, P1 κs → P2 κs.
+Global Instance spec_equiv : Equiv spec := λ P1 P2, ∀ κs, P1 κs ↔ P2 κs.
+
+Canonical Structure specO := list seq_label -d> PropO.
+
+Definition snil : spec :=
+  λ κs, κs = [].
+
+Definition scons (l : seq_label) (P : spec) : spec :=
+  λ κs, κs = [] ∨ ∃ κs', κs = l::κs' ∧ (κs' = [] ∨ P κs').
+
+Definition sapp (ls : list seq_label) (P : spec) : spec :=
+  foldr scons P ls.
+
+Definition sexists {A} (P : A → spec) : spec :=
+  λ κs, ∃ a, P a κs.
+
+Definition sif (C : Prop) (P1 : spec) (P2 : spec) : spec :=
+  λ κs, (C ∧ P1 κs) ∨ (¬ C ∧ P2 κs).
+
+Definition srec (P : spec → spec) : spec :=
+  least_fixpoint P.
+
+Ltac spec_unfold :=
+  unfold subseteq, spec_subseteq, equiv, spec_equiv, scons, snil, sexists, sif in *.
+Ltac spec_solver := spec_unfold; naive_solver.
+
+Global Instance spec_equiv_equiv : Equivalence (≡@{spec}).
+Proof. constructor => ? *; spec_solver. Qed.
+Global Instance spec_subseteq_preorder : PreOrder (⊆@{spec}).
+Proof. constructor => ? *; spec_solver. Qed.
+Global Instance spec_subseteq_equiv_proper : Proper (equiv ==> equiv ==> iff) (⊆@{spec}).
+Proof. move => ??????. spec_solver. Qed.
+
+Lemma sif_true (P : Prop) Pκs1 Pκs2: P → sif P Pκs1 Pκs2 ≡ Pκs1.
+Proof. spec_solver. Qed.
+Lemma sif_false (P : Prop) Pκs1 Pκs2: ¬ P → sif P Pκs1 Pκs2 ≡ Pκs2.
+Proof. spec_solver. Qed.
+
+
+(* This is unsafe due to the κs' = [] ∨ ... in scons. *)
+Global Instance simpl_and_scons_subseteq κ1 κ2 Pκs1 Pκs2:
+  SimplAndUnsafe true (scons κ1 Pκs1 ⊆ scons κ2 Pκs2) (λ T, κ1 = κ2 ∧ Pκs1 ⊆ Pκs2 ∧ T).
+Proof. move => ?. spec_solver. Qed.
+
+(* Unsafe since there might be multiple different choices for x for different traces. *)
+Global Instance simpl_and_scons_subseteq_sexists {A} κ1 Pκs1 Pκs2:
+  SimplAndUnsafe true (scons κ1 Pκs1 ⊆ sexists Pκs2) (λ T, ∃ x : A, scons κ1 Pκs1 ⊆ Pκs2 x ∧ T).
+Proof. move => ?. spec_solver. Qed.
+
+Global Instance simpl_and_scons_subseteq_srec κ1 Pκs1 Prec `{!MonoPred Prec}:
+  SimplAnd (scons κ1 Pκs1 ⊆ srec Prec) (λ T, scons κ1 Pκs1 ⊆ Prec (srec Prec) ∧ T).
+Proof. split; move => [??]; (split; [|done]) => ??; apply/least_fixpoint_unfold; spec_solver. Qed.
+
+Global Instance simpl_and_spec_subseteq_evar (Pκs1 Pκs2 : spec) `{!IsProtected Pκs1}:
+  SimplAndUnsafe true (Pκs1 ⊆ Pκs2) (λ T, Pκs1 = Pκs2 ∧ T).
+Proof. move => ?. spec_solver. Qed.
